Move misc lemmas, small fixes

Certification/Normalized_Zone_Semantics_Certification_Impl.thy
@@ -9,296 +9,8 @@ theory Normalized_Zone_Semantics_Certification_Impl
     Deadlock.Deadlock_Impl
     TA_Library.More_Methods
     "HOL-Library.Rewrite"
+    Unreachability_TA_Misc
 begin
-
-paragraph \<open>Misc\<close>
-
-lemma (in Graph_Defs) run_first_reaches:
-  "pred_stream (reaches x) xs" if "run (x ## xs)"
-proof -
-  from that obtain a where "run (a ## xs)" "reaches x a"
-    by auto
-  then show ?thesis
-    by (coinduction arbitrary: a xs rule: stream_pred_coinduct) (auto 4 3 elim: run.cases)
-qed
-
-lemma (in Graph_Start_Defs) run_reachable:
-  "pred_stream reachable xs" if "run (s\<^sub>0 ## xs)"
-  using run_first_reaches[OF that] unfolding reachable_def .
-
-lemma pred_stream_stream_all2_combine:
-  assumes "pred_stream P xs" "stream_all2 Q xs ys" "\<And>x y. P x \<Longrightarrow> Q x y \<Longrightarrow> R x y"
-  shows "stream_all2 R xs ys"
-  using assms by (auto intro: stream_all2_combine simp: stream.pred_rel eq_onp_def)
-
-lemma stream_all2_pred_stream_combine:
-  assumes "stream_all2 Q xs ys" "pred_stream P ys" "\<And>x y. Q x y \<Longrightarrow> P y \<Longrightarrow> R x y"
-  shows "stream_all2 R xs ys"
-  using assms by (auto intro: stream_all2_combine simp: stream.pred_rel eq_onp_def)
-
-lemma map_set_rel:
-  assumes "list_all P xs" "(f, g) \<in> {(xs, ys). xs = ys \<and> P xs} \<rightarrow> B"
-  shows "(map f xs, g ` set xs) \<in> \<langle>B\<rangle>list_set_rel"
-  unfolding list_set_rel_def
-  apply (rule relcompI[where b = "map g xs"])
-  apply parametricity
-  using assms unfolding list_rel_def list_all_iff by (auto intro: list.rel_refl_strong)
-
-context TA_Start
-begin
-
-(* XXX This is in Normalized_Zone_Semantics_Impl but in the wrong context *)
-lemma V_I:
-  assumes "\<forall> i \<in> {1..<Suc n}. M 0 i \<le> 0"
-  shows "[M]\<^bsub>v,n\<^esub> \<subseteq> V"
-  unfolding V_def DBM_zone_repr_def
-proof (safe, goal_cases)
-  case prems: (1 u i)
-  then have "v i = i"
-    using X_alt_def X_def triv_numbering by blast
-  with prems have "v i > 0" "v i \<le> n" by auto
-  with prems have "dbm_entry_val u None (Some i) (M 0 (v i))"
-    unfolding DBM_val_bounded_def by auto
-  moreover from assms \<open>v i > 0\<close> \<open>v i \<le> n\<close> have "M 0 (v i) \<le> 0" by auto
-  ultimately
-  show ?case
-    apply (cases "M 0 (v i)")
-    unfolding neutral less_eq dbm_le_def
-    by (auto elim!: dbm_lt.cases simp: \<open>v i = i\<close>)
-qed
-
-end
-
-lemma Simulation_Composition:
-  fixes A B C
-  assumes
-    "Simulation A B sim1" "Simulation B C sim2" "\<And>a c. (\<exists> b. sim1 a b \<and> sim2 b c) \<longleftrightarrow> sim a c"
-  shows "Simulation A C sim"
-proof -
-  interpret A: Simulation A B sim1
-    by (rule assms)
-  interpret B: Simulation B C sim2
-    by (rule assms)
-  show ?thesis
-    by standard (auto dest!: B.A_B_step A.A_B_step simp: assms(3)[symmetric])
-qed
-
-lemma fold_generalize_start:
-  assumes "\<And>a. P a \<Longrightarrow> Q (fold g xs a)" "P a"
-  shows "Q (fold g xs a)"
-  using assms by auto
-
-definition
-  "set_of_list xs = SPEC (\<lambda>S. set xs = S)"
-
-(* XXX Move *)
-lemma set_of_list_hnr:
-  "(return o id, set_of_list) \<in> (list_assn A)\<^sup>d \<rightarrow>\<^sub>a lso_assn A"
-  unfolding set_of_list_def lso_assn_def hr_comp_def br_def by sepref_to_hoare sep_auto
-
-lemma set_of_list_alt_def:
-  "set_of_list = RETURN o set"
-  unfolding set_of_list_def by auto
-
-lemmas set_of_list_hnr' = set_of_list_hnr[unfolded set_of_list_alt_def]
-
-
-lemmas amtx_copy_hnr = amtx_copy_hnr[unfolded op_mtx_copy_def, folded COPY_def[abs_def]]
-
-lemma lso_op_set_is_empty_hnr[sepref_fr_rules]:
-  "(return o (\<lambda>xs. xs = []), RETURN o op_set_is_empty) \<in> (lso_assn AA)\<^sup>k \<rightarrow>\<^sub>a bool_assn"
-  unfolding lso_assn_def hr_comp_def br_def by sepref_to_hoare sep_auto
-
-context
-  fixes n :: nat
-begin
-
-qualified definition
-  "dbm_tab M \<equiv> \<lambda> (i, j). if i \<le> n \<and> j \<le> n then M ! ((n + 1) * i + j) else 0"
-
-private lemma
-  shows mtx_nonzero_dbm_tab_1: "(a, b) \<in> mtx_nonzero (dbm_tab M) \<Longrightarrow> a < Suc n"
-    and mtx_nonzero_dbm_tab_2: "(a, b) \<in> mtx_nonzero (dbm_tab M) \<Longrightarrow> b < Suc n"
-  unfolding mtx_nonzero_def dbm_tab_def by (auto split: if_split_asm)
-
-definition
-  "list_to_dbm M = op_amtx_new (Suc n) (Suc n) (dbm_tab M)"
-
-lemma [sepref_fr_rules]:
-  "(return o dbm_tab, RETURN o PR_CONST dbm_tab) \<in> id_assn\<^sup>k \<rightarrow>\<^sub>a pure (nat_rel \<times>\<^sub>r nat_rel \<rightarrow> Id)"
-  by sepref_to_hoare sep_auto
-
-lemmas [sepref_opt_simps] = dbm_tab_def
-
-sepref_register dbm_tab
-
-sepref_definition list_to_dbm_impl
-  is "RETURN o PR_CONST list_to_dbm" :: "id_assn\<^sup>k \<rightarrow>\<^sub>a mtx_assn n"
-  supply mtx_nonzero_dbm_tab_1[simp] mtx_nonzero_dbm_tab_2[simp]
-  unfolding PR_CONST_def list_to_dbm_def by sepref
-
-lemma the_pure_Id:
-  "the_pure (\<lambda>a c. \<up> (c = a)) = Id"
-  by (subst is_pure_the_pure_id_eq) (auto simp: pure_def intro: is_pureI)
-
-lemma of_list_list_to_dbm:
-  "(Array.of_list, (RETURN \<circ>\<circ> PR_CONST) list_to_dbm)
-  \<in> [\<lambda>a. length a = Suc n * Suc n]\<^sub>a id_assn\<^sup>k \<rightarrow> mtx_assn n"
-  apply sepref_to_hoare
-  apply sep_auto
-  unfolding amtx_assn_def hr_comp_def IICF_Array_Matrix.is_amtx_def
-  apply (sep_auto eintros del: exI)
-  subgoal for xs p
-    apply (rule exI[where x = "list_to_dbm xs"])
-    apply (rule exI[where x = xs])
-    apply (sep_auto simp: list_to_dbm_def dbm_tab_def the_pure_Id)
-     apply (simp add: algebra_simps; fail)
-    apply sep_auto
-    done
-  done
-
-end
-
-definition
-  "array_freeze a = do {xs \<leftarrow> Array.freeze a; Heap_Monad.return (IArray xs)}"
-
-definition
-  "array_unfreeze a = Array.of_list (IArray.list_of a)"
-
-definition
-  "iarray_mtx_rel n m c a \<equiv>
-    IArray.length a = n * m
-  \<and> (\<forall>i<n.\<forall>j<m. c (i, j) = IArray.sub a (i * m + j))
-  \<and> (\<forall>i j. i \<ge> n \<or> j \<ge> m \<longrightarrow> c (i, j) = 0)"
-
-lemma iarray_mtx_rel_is_amtx:
-  "x \<mapsto>\<^sub>a IArray.list_of a \<Longrightarrow>\<^sub>A IICF_Array_Matrix.is_amtx n m c x" if "iarray_mtx_rel n m c a"
-  using that unfolding is_amtx_def iarray_mtx_rel_def by simp solve_entails
-
-lemma array_unfreeze_ht:
-  "<emp> array_unfreeze a <amtx_assn n m id_assn c>" if "iarray_mtx_rel n m c a"
-  using that unfolding array_unfreeze_def amtx_assn_def by (sep_auto intro: iarray_mtx_rel_is_amtx)
-
-lemma array_freeze_ht:
-  "<amtx_assn n m id_assn c a> array_freeze a <\<lambda>a. \<up>(iarray_mtx_rel n m c a)>\<^sub>t"
-  unfolding array_freeze_def amtx_assn_def iarray_mtx_rel_def is_amtx_def
-  by (sep_auto intro: iarray_mtx_rel_is_amtx)
-
-
-datatype ('a, 'b) frozen_hm =
-  Frozen_Hash_Map (array_of_hm: "('a, 'b) list_map iarray") (size_of_hm: nat)
-
-definition diff_array_freeze :: "'a array \<Rightarrow> 'a iarray" where
-  "diff_array_freeze a = IArray (list_of_array a)"
-
-definition hm_freeze where
-  "hm_freeze \<equiv> \<lambda>hm. case hm of Impl_Array_Hash_Map.HashMap a _
-    \<Rightarrow> Frozen_Hash_Map (diff_array_freeze a) (array_length a)"
-
-definition frozen_hm_lookup where
-  "frozen_hm_lookup \<equiv> \<lambda>key hm.
-    case hm of Frozen_Hash_Map a n \<Rightarrow>
-      let
-        code = bounded_hashcode_nat n key;
-        bucket = IArray.sub a code
-      in
-        list_map_lookup (=) key bucket
-  "
-
-lemma list_of_array_nth:
-  "list_of_array a ! n = array_get a n"
-  by (cases a) simp
-
-lemma frozen_hm_lookup_hm_freeze:
-  "frozen_hm_lookup k (hm_freeze m) = Impl_Array_Hash_Map.ahm_lookup (=) bounded_hashcode_nat k m"
-proof -
-  obtain a n where "m = Impl_Array_Hash_Map.HashMap a n"
-    by (cases m) auto
-  have "IArray.sub (diff_array_freeze a) i = array_get a i" for i
-    unfolding diff_array_freeze_def by (simp add: list_of_array_nth)
-  then show ?thesis
-    unfolding frozen_hm_lookup_def \<open>m = _\<close> hm_freeze_def by simp
-qed
-
-context
-  fixes M :: "('a :: hashable * 'b) list"
-begin
-
-definition "map_of_list = fold (\<lambda>(k, v) a. a(k \<mapsto> v)) M Map.empty"
-
-lemma [autoref_rules]:
-  "(M, M) \<in> \<langle>Id \<times>\<^sub>r Id\<rangle>list_rel"
-  by simp
-
-schematic_goal M_impl:
-  "(?M::?'c, map_of_list:::\<^sub>r\<langle>Id,Id\<rangle>dflt_ahm_rel) \<in> ?R"
-  unfolding map_of_list_def
-  apply (autoref (trace))
-  done
-
-concrete_definition hashmap_of_list uses M_impl
-
-definition
-  "frozen_hm_of_list \<equiv> hm_freeze hashmap_of_list"
-
-theorem hashmap_of_list_lookup:
-  "(\<lambda>k. Impl_Array_Hash_Map.ahm_lookup (=) bounded_hashcode_nat k hashmap_of_list, map_of_list)
-  \<in> Id \<rightarrow> \<langle>Id\<rangle>option_rel" (is "(\<lambda>k. ?f k hashmap_of_list, _) \<in> ?R")
-proof -
-  have *: "(?f, Intf_Map.op_map_lookup) \<in> Id \<rightarrow> ahm_map_rel' bounded_hashcode_nat \<rightarrow> Id"
-    using Impl_Array_Hash_Map.ahm_lookup_impl[OF hashable_bhc_is_bhc] by simp
-  { fix k :: 'a
-    have "abstract_bounded_hashcode Id bounded_hashcode_nat = bounded_hashcode_nat"
-      unfolding abstract_bounded_hashcode_def by (intro ext) auto
-    from hashmap_of_list.refine obtain hm where
-      "(hashmap_of_list, hm) \<in> \<langle>Id, Id\<rangle>ahm_map_rel"
-      "(hm, map_of_list) \<in> ahm_map_rel' bounded_hashcode_nat"
-      unfolding ahm_rel_def by (clarsimp simp: \<open>_ = bounded_hashcode_nat\<close>)
-    with * have "?f k hm = Intf_Map.op_map_lookup k map_of_list"
-      by (auto dest!: fun_relD)
-    with \<open>(hashmap_of_list, hm) \<in> _\<close> have "?f k hashmap_of_list = map_of_list k"
-      unfolding ahm_map_rel_def array_rel_def by clarsimp
-  }
-  then show ?thesis
-    by simp
-qed
-
-theorem frozen_hm_of_list_lookup:
-  "(\<lambda>k. frozen_hm_lookup k frozen_hm_of_list, map_of_list) \<in> Id \<rightarrow> \<langle>Id\<rangle>option_rel"
-  using hashmap_of_list_lookup unfolding frozen_hm_of_list_def
-  by (simp add: frozen_hm_lookup_hm_freeze)
-
-end
-
-
-definition
-  "array_all2 n P as bs \<equiv> \<forall>i < n. P (IArray.sub as i) (IArray.sub bs i)"
-
-lemma iarray_mtx_relD:
-  assumes "iarray_mtx_rel n m M a" "i < n" "j < m"
-  shows "M (i, j) = IArray.sub a (i * m + j)"
-  using assms unfolding iarray_mtx_rel_def by auto
-
-lemma array_all2_iff_pointwise_cmp:
-  assumes "iarray_mtx_rel (Suc n) (Suc n) M a" "iarray_mtx_rel (Suc n) (Suc n) M' b"
-  shows "array_all2 (Suc n * Suc n) P a b \<longleftrightarrow> pointwise_cmp P n (curry M) (curry M')"
-proof -
-  have *: \<open>i + i * n + j < Suc (n + (n + n * n))\<close> if \<open>i \<le> n\<close> and \<open>j \<le> n\<close> for i j :: \<open>nat\<close>
-    using that by (simp add: algebra_simps) (intro le_imp_less_Suc add_mono; simp)
-  have **: "\<exists>i \<le> n. \<exists>j \<le> n. k = i + i * n + j" if "k < Suc n * Suc n" for k
-    apply (inst_existentials "k div Suc n" "k mod Suc n")
-    subgoal
-      by (meson less_Suc_eq_le less_mult_imp_div_less that)
-    subgoal
-      by simp
-    subgoal
-      by (metis div_mod_decomp mult_Suc_right)
-    done
-  from assms show ?thesis
-    unfolding pointwise_cmp_def array_all2_def
-    by (auto dest: *[simplified] **[simplified] simp: iarray_mtx_relD)
-qed
-
 
 context TA_Impl
 begin
@@ -594,7 +306,7 @@ lemma P_impl_refine:
 
 lemmas [safe_constraint_rules] = location_assn_constraints
 
-end (* TA Impl Precise *)
+end (* TA Impl Ext *)
 
 
 paragraph \<open>Deriving the Main Simulation Theorems\<close>
@@ -775,8 +487,7 @@ lemmas [sepref_fr_rules] = set_of_list_hnr'
 lemma IArray_list_to_dbm_rel[param]:
   "(IArray, list_to_dbm n)
   \<in> {(xs, ys). xs = ys \<and> length xs = Suc n * Suc n} \<rightarrow> {(a, b). iarray_mtx_rel (Suc n) (Suc n) b a}"
-  unfolding list_to_dbm_def op_amtx_new_def iarray_mtx_rel_def
-    Normalized_Zone_Semantics_Certification_Impl.dbm_tab_def
+  unfolding list_to_dbm_def op_amtx_new_def iarray_mtx_rel_def Unreachability_TA_Misc.dbm_tab_def
   by (auto simp: algebra_simps)
 
 lemma IArray_list_to_dbm_rel':
@@ -1102,20 +813,6 @@ interpretation
     and L = "set L"
     and M = M
   apply standard
-                      apply (rule HOL.refl; fail)
-                      apply (rule dbm_subset_refl; fail)
-                      apply (rule dbm_subset_trans; assumption)
-  subgoal (* succs correct *)
-    unfolding succs_precise_def op_precise.E_from_op_empty_def op_precise.E_from_op_def
-    apply (auto dest!: trans_impl_trans_of)
-    apply (auto dest!: trans_of_trans_impl)
-    apply (intro exI conjI, erule image_eqI[rotated])
-     apply auto
-    done
-  subgoal (* P correct *)
-    by (auto dest: P_correct)
-  subgoal (* F mono *)
-    by (rule F_mono)
   subgoal (* L finite *)
     ..
   subgoal (* M finite *)
@@ -1129,25 +826,41 @@ interpretation
     by (rule L_list_hnr) *)
       (* subgoal (* M refine *)
     unfolding PR_CONST_def by (rule M_table.refine) *)
+  subgoal (* succs correct *)
+    unfolding succs_precise_def op_precise.E_from_op_empty_def op_precise.E_from_op_def
+    apply (auto dest!: trans_impl_trans_of)
+    apply (auto dest!: trans_of_trans_impl)
+    apply (intro exI conjI, erule image_eqI[rotated])
+     apply auto
+    done
+  subgoal (* P correct *)
+    by (auto dest: P_correct)
   subgoal (* key refine *)
     by sepref_to_hoare sep_auto
-           apply (rule amtx_copy_hnr; fail)
+  apply (rule amtx_copy_hnr; fail) (* COPY implementation for dbms *)
   subgoal (* P refine *)
     by (rule P_impl_refine)
   subgoal (* F refine *)
     by (rule F_impl)
   subgoal (* succs refine *)
     using succs_precise_impl_refine unfolding b_assn_pure_conv .
-       apply (rule dbm_subset_impl.refine; fail)
-        apply (rule location_assn_constraints; fail)+
+  apply (rule location_assn_constraints; fail)+ (* location assn is correct *)
+  subgoal (* init loc refine *)
+    using init_impl states'_states by sepref_to_hoare sep_auto
+  (* init dbm refine *)
+         apply (unfold PR_CONST_def, rule init_dbm_impl.refine; fail)
+  (* dbm subset relation is an ordering *)
+  apply (rule HOL.refl; fail)
+  apply (rule dbm_subset_refl; fail)
+  apply (rule dbm_subset_trans; assumption)
+  subgoal (* F mono *)
+    by (rule F_mono)
   subgoal (* E_precise mono *)
     by (auto dest: op_precise.E_from_op_empty_mono')
   subgoal (* E_precise invariant *)
     by (clarsimp simp: op_precise.E_from_op_empty_def, frule op_precise.E_from_op_wf_state[rotated])
       (auto dest: E_from_op_states simp: wf_state_def)
-  subgoal (* init loc refine *)
-    using init_impl states'_states by sepref_to_hoare sep_auto
-     apply (unfold PR_CONST_def, rule init_dbm_impl.refine; fail)
+  apply (rule dbm_subset_impl.refine; fail) (* dbm subset refinement *)
   done
 
 lemmas reachability_impl = Reachability_Impl_axioms
@@ -1253,7 +966,7 @@ definition
     succsi = succs_precise'_impl;
     M_table = M_table
   in
-    certify_unreachable_impl Fi Pi copyi Lei succsi l\<^sub>0i s\<^sub>0i L_list M_table splitteri"
+    certify_unreachable_impl Fi Pi copyi succsi l\<^sub>0i s\<^sub>0i Lei L_list M_table splitteri"
 
 lemma unreachability_checker_alt_def:
   "unreachability_checker \<equiv>
@@ -1267,7 +980,7 @@ lemma unreachability_checker_alt_def:
     succsi = succs_precise'_impl
   in do {
     M_table \<leftarrow> M_table;
-    certify_unreachable_impl_inner Fi Pi copyi Lei succsi l\<^sub>0i s\<^sub>0i splitteri L_list M_table
+    certify_unreachable_impl_inner Fi Pi copyi succsi l\<^sub>0i s\<^sub>0i Lei splitteri L_list M_table
   }"
   unfolding unreachability_checker_def certify_unreachable_impl_def Let_def .
 
@@ -1288,7 +1001,7 @@ definition
     succsi = succs_precise'_impl;
     M_table = M_table
   in
-    certify_unreachable_impl2 Fi Pi copyi Lei succsi l\<^sub>0i s\<^sub>0i splitteri L_list M_table"
+    certify_unreachable_impl2 Fi Pi copyi succsi l\<^sub>0i s\<^sub>0i Lei splitteri L_list M_table"
 
 lemmas unreachability_checker2_refine = certify_unreachable_impl2_refine[
     of L_list M_table splitter splitteri,
@@ -1369,9 +1082,6 @@ interpretation
     and L = "set L"
     and M = "\<lambda>x. case M2 x of None \<Rightarrow> {} | Some S \<Rightarrow> S"
   apply standard
-                      apply (rule HOL.refl; fail)
-                      apply (rule dbm_subset_refl; fail)
-                      apply (rule dbm_subset_trans; assumption)
   subgoal (* succs correct *)
     unfolding succs_precise_def op_precise.E_from_op_empty_def op_precise.E_from_op_def
     apply (auto dest!: trans_impl_trans_of)
@@ -1379,6 +1089,10 @@ interpretation
     apply (intro exI conjI, erule image_eqI[rotated])
      apply auto
     done
+  (* dbm subset relation is an ordering *)
+  apply (rule HOL.refl; fail)
+  apply (rule dbm_subset_refl; fail)
+  apply (rule dbm_subset_trans; assumption)
   subgoal (* P correct *)
     by (auto dest: P_correct)
   subgoal (* F mono *)
